- Adapted islaris to the new trace syntax for the enumerate types and values produced by the new isla-footprint - Changed Makefile instructions for coq-bbv for `make deps`: use coq-bbv.1.4 instead of 1.3 and install via opam

instructions/memcpy_riscv64/a8.v
@@ -14,27 +14,27 @@ Definition a8 : isla_trace :=
   Assume (AExp_Binop (Eq) (AExp_Unop (Extract 2%N 2%N) (AExp_Val (AVal_Var "misa" [Field "bits"]) Mk_annot) Mk_annot) (AExp_Val (AVal_Bits (BV 1%N 0x1%Z)) Mk_annot) Mk_annot) Mk_annot :t:
   Smt (DeclareConst 1%Z (Ty_BitVec 64%N)) Mk_annot :t:
   Assume (AExp_Binop (Eq) (AExp_Manyop (Bvmanyarith Bvand) [AExp_Val (AVal_Var "mstatus" [Field "bits"]) Mk_annot; AExp_Val (AVal_Bits (BV 64%N 0x20000%Z)) Mk_annot] Mk_annot) (AExp_Val (AVal_Bits (BV 64%N 0x0%Z)) Mk_annot) Mk_annot) Mk_annot :t:
-  Smt (DeclareConst 6%Z (Ty_Enum (Mk_enum_id 3%nat))) Mk_annot :t:
+  Smt (DeclareConst 2%Z (Ty_Enum "Privilege")) Mk_annot :t:
   Assume (AExp_Binop (Eq) (AExp_Val (AVal_Var "cur_privilege" []) Mk_annot) (AExp_Val (AVal_Var "Machine" []) Mk_annot) Mk_annot) Mk_annot :t:
-  Smt (DeclareConst 7%Z (Ty_BitVec 64%N)) Mk_annot :t:
+  Smt (DeclareConst 3%Z (Ty_BitVec 64%N)) Mk_annot :t:
   Assume (AExp_Binop ((Bvcomp Bvuge)) (AExp_Val (AVal_Var "x10" []) Mk_annot) (AExp_Val (AVal_Var "rv_ram_base" []) Mk_annot) Mk_annot) Mk_annot :t:
   Assume (AExp_Binop ((Bvcomp Bvult)) (AExp_Val (AVal_Var "x10" []) Mk_annot) (AExp_Manyop (Bvmanyarith Bvadd) [AExp_Val (AVal_Var "rv_ram_base" []) Mk_annot; AExp_Val (AVal_Var "rv_ram_size" []) Mk_annot] Mk_annot) Mk_annot) Mk_annot :t:
-  Smt (DeclareConst 8%Z (Ty_BitVec 64%N)) Mk_annot :t:
-  ReadReg "PC" [] (RegVal_Base (Val_Symbolic 8%Z)) Mk_annot :t:
-  Smt (DefineConst 9%Z (Manyop (Bvmanyarith Bvadd) [Val (Val_Symbolic 8%Z) Mk_annot; Val (Val_Bits (BV 64%N 0x4%Z)) Mk_annot] Mk_annot)) Mk_annot :t:
-  ReadReg "x10" [] (RegVal_Base (Val_Symbolic 7%Z)) Mk_annot :t:
-  Smt (DefineConst 21%Z (Manyop (Bvmanyarith Bvadd) [Val (Val_Symbolic 7%Z) Mk_annot; Val (Val_Bits (BV 64%N 0x0%Z)) Mk_annot] Mk_annot)) Mk_annot :t:
+  Smt (DeclareConst 4%Z (Ty_BitVec 64%N)) Mk_annot :t:
+  ReadReg "PC" [] (RegVal_Base (Val_Symbolic 4%Z)) Mk_annot :t:
+  Smt (DefineConst 5%Z (Manyop (Bvmanyarith Bvadd) [Val (Val_Symbolic 4%Z) Mk_annot; Val (Val_Bits (BV 64%N 0x4%Z)) Mk_annot] Mk_annot)) Mk_annot :t:
+  ReadReg "x10" [] (RegVal_Base (Val_Symbolic 3%Z)) Mk_annot :t:
+  Smt (DefineConst 6%Z (Manyop (Bvmanyarith Bvadd) [Val (Val_Symbolic 3%Z) Mk_annot; Val (Val_Bits (BV 64%N 0x0%Z)) Mk_annot] Mk_annot)) Mk_annot :t:
   ReadReg "mstatus" [] (RegVal_Struct [("bits", RegVal_Base (Val_Symbolic 1%Z))]) Mk_annot :t:
-  ReadReg "cur_privilege" [] (RegVal_Base (Val_Symbolic 6%Z)) Mk_annot :t:
-  Smt (DeclareConst 29%Z (Ty_BitVec 64%N)) Mk_annot :t:
-  ReadReg "satp" [] (RegVal_Base (Val_Symbolic 29%Z)) Mk_annot :t:
-  Smt (DeclareConst 47%Z (Ty_BitVec 64%N)) Mk_annot :t:
-  ReadReg "x13" [] (RegVal_Base (Val_Symbolic 47%Z)) Mk_annot :t:
-  Smt (DefineConst 50%Z (Unop (Extract 7%N 0%N) (Val (Val_Symbolic 47%Z) Mk_annot) Mk_annot)) Mk_annot :t:
-  Smt (DefineConst 56%Z (Unop (ZeroExtend 64%N) (Val (Val_Symbolic 21%Z) Mk_annot) Mk_annot)) Mk_annot :t:
-  Smt (DefineConst 62%Z (Unop (ZeroExtend 64%N) (Val (Val_Symbolic 21%Z) Mk_annot) Mk_annot)) Mk_annot :t:
-  Smt (DeclareConst 66%Z Ty_Bool) Mk_annot :t:
-  WriteMem (RegVal_Base (Val_Symbolic 66%Z)) (RegVal_Base (Val_Enum ((Mk_enum_id 2%nat), Mk_enum_ctor 0%nat))) (RegVal_Base (Val_Symbolic 21%Z)) (RegVal_Base (Val_Symbolic 50%Z)) 1%N None Mk_annot :t:
-  WriteReg "PC" [] (RegVal_Base (Val_Symbolic 9%Z)) Mk_annot :t:
+  ReadReg "cur_privilege" [] (RegVal_Base (Val_Symbolic 2%Z)) Mk_annot :t:
+  Smt (DeclareConst 14%Z (Ty_BitVec 64%N)) Mk_annot :t:
+  ReadReg "satp" [] (RegVal_Base (Val_Symbolic 14%Z)) Mk_annot :t:
+  Smt (DeclareConst 19%Z (Ty_BitVec 64%N)) Mk_annot :t:
+  ReadReg "x13" [] (RegVal_Base (Val_Symbolic 19%Z)) Mk_annot :t:
+  Smt (DefineConst 20%Z (Unop (Extract 7%N 0%N) (Val (Val_Symbolic 19%Z) Mk_annot) Mk_annot)) Mk_annot :t:
+  Smt (DefineConst 23%Z (Unop (ZeroExtend 64%N) (Val (Val_Symbolic 6%Z) Mk_annot) Mk_annot)) Mk_annot :t:
+  Smt (DefineConst 29%Z (Unop (ZeroExtend 64%N) (Val (Val_Symbolic 6%Z) Mk_annot) Mk_annot)) Mk_annot :t:
+  Smt (DeclareConst 33%Z Ty_Bool) Mk_annot :t:
+  WriteMem (RegVal_Base (Val_Symbolic 33%Z)) (RegVal_Poison) (RegVal_Base (Val_Symbolic 6%Z)) (RegVal_Base (Val_Symbolic 20%Z)) 1%N None Mk_annot :t:
+  WriteReg "PC" [] (RegVal_Base (Val_Symbolic 5%Z)) Mk_annot :t:
   tnil
 .
