instructions/riscv64_test/a8.v
@@ -14,27 +14,27 @@ Definition a8 : isla_trace :=
   Assume (AExp_Binop (Eq) (AExp_Unop (Extract 2%N 2%N) (AExp_Val (AVal_Var "misa" [Field "bits"]) Mk_annot) Mk_annot) (AExp_Val (AVal_Bits (BV 1%N 0x1%Z)) Mk_annot) Mk_annot) Mk_annot :t:
   Smt (DeclareConst 1%Z (Ty_BitVec 64%N)) Mk_annot :t:
   Assume (AExp_Binop (Eq) (AExp_Manyop (Bvmanyarith Bvand) [AExp_Val (AVal_Var "mstatus" [Field "bits"]) Mk_annot; AExp_Val (AVal_Bits (BV 64%N 0x20000%Z)) Mk_annot] Mk_annot) (AExp_Val (AVal_Bits (BV 64%N 0x0%Z)) Mk_annot) Mk_annot) Mk_annot :t:
-  Smt (DeclareConst 6%Z (Ty_Enum (Mk_enum_id 3%nat))) Mk_annot :t:
+  Smt (DeclareConst 2%Z (Ty_Enum "Privilege")) Mk_annot :t:
   Assume (AExp_Binop (Eq) (AExp_Val (AVal_Var "cur_privilege" []) Mk_annot) (AExp_Val (AVal_Var "Machine" []) Mk_annot) Mk_annot) Mk_annot :t:
-  Smt (DeclareConst 7%Z (Ty_BitVec 64%N)) Mk_annot :t:
+  Smt (DeclareConst 3%Z (Ty_BitVec 64%N)) Mk_annot :t:
   Assume (AExp_Binop (Eq) (AExp_Unop (Extract 2%N 0%N) (AExp_Val (AVal_Var "x2" []) Mk_annot) Mk_annot) (AExp_Val (AVal_Bits (BV 3%N 0x0%Z)) Mk_annot) Mk_annot) Mk_annot :t:
   Assume (AExp_Binop ((Bvcomp Bvuge)) (AExp_Manyop (Bvmanyarith Bvadd) [AExp_Val (AVal_Var "x2" []) Mk_annot; AExp_Val (AVal_Bits (BV 64%N 0x8%Z)) Mk_annot] Mk_annot) (AExp_Val (AVal_Var "rv_ram_base" []) Mk_annot) Mk_annot) Mk_annot :t:
   Assume (AExp_Binop ((Bvcomp Bvult)) (AExp_Manyop (Bvmanyarith Bvadd) [AExp_Val (AVal_Var "x2" []) Mk_annot; AExp_Val (AVal_Bits (BV 64%N 0x8%Z)) Mk_annot] Mk_annot) (AExp_Manyop (Bvmanyarith Bvadd) [AExp_Val (AVal_Var "rv_ram_base" []) Mk_annot; AExp_Val (AVal_Var "rv_ram_size" []) Mk_annot] Mk_annot) Mk_annot) Mk_annot :t:
-  Smt (DeclareConst 8%Z (Ty_BitVec 64%N)) Mk_annot :t:
-  ReadReg "PC" [] (RegVal_Base (Val_Symbolic 8%Z)) Mk_annot :t:
-  Smt (DefineConst 9%Z (Manyop (Bvmanyarith Bvadd) [Val (Val_Symbolic 8%Z) Mk_annot; Val (Val_Bits (BV 64%N 0x4%Z)) Mk_annot] Mk_annot)) Mk_annot :t:
-  ReadReg "x2" [] (RegVal_Base (Val_Symbolic 7%Z)) Mk_annot :t:
-  Smt (DefineConst 21%Z (Manyop (Bvmanyarith Bvadd) [Val (Val_Symbolic 7%Z) Mk_annot; Val (Val_Bits (BV 64%N 0x8%Z)) Mk_annot] Mk_annot)) Mk_annot :t:
+  Smt (DeclareConst 4%Z (Ty_BitVec 64%N)) Mk_annot :t:
+  ReadReg "PC" [] (RegVal_Base (Val_Symbolic 4%Z)) Mk_annot :t:
+  Smt (DefineConst 5%Z (Manyop (Bvmanyarith Bvadd) [Val (Val_Symbolic 4%Z) Mk_annot; Val (Val_Bits (BV 64%N 0x4%Z)) Mk_annot] Mk_annot)) Mk_annot :t:
+  ReadReg "x2" [] (RegVal_Base (Val_Symbolic 3%Z)) Mk_annot :t:
+  Smt (DefineConst 6%Z (Manyop (Bvmanyarith Bvadd) [Val (Val_Symbolic 3%Z) Mk_annot; Val (Val_Bits (BV 64%N 0x8%Z)) Mk_annot] Mk_annot)) Mk_annot :t:
   ReadReg "mstatus" [] (RegVal_Struct [("bits", RegVal_Base (Val_Symbolic 1%Z))]) Mk_annot :t:
-  ReadReg "cur_privilege" [] (RegVal_Base (Val_Symbolic 6%Z)) Mk_annot :t:
-  Smt (DeclareConst 35%Z (Ty_BitVec 64%N)) Mk_annot :t:
-  ReadReg "satp" [] (RegVal_Base (Val_Symbolic 35%Z)) Mk_annot :t:
-  Smt (DeclareConst 53%Z (Ty_BitVec 64%N)) Mk_annot :t:
-  ReadReg "x11" [] (RegVal_Base (Val_Symbolic 53%Z)) Mk_annot :t:
-  Smt (DefineConst 61%Z (Unop (ZeroExtend 64%N) (Val (Val_Symbolic 21%Z) Mk_annot) Mk_annot)) Mk_annot :t:
-  Smt (DefineConst 67%Z (Unop (ZeroExtend 64%N) (Val (Val_Symbolic 21%Z) Mk_annot) Mk_annot)) Mk_annot :t:
-  Smt (DeclareConst 71%Z Ty_Bool) Mk_annot :t:
-  WriteMem (RegVal_Base (Val_Symbolic 71%Z)) (RegVal_Base (Val_Enum ((Mk_enum_id 2%nat), Mk_enum_ctor 0%nat))) (RegVal_Base (Val_Symbolic 21%Z)) (RegVal_Base (Val_Symbolic 53%Z)) 8%N None Mk_annot :t:
-  WriteReg "PC" [] (RegVal_Base (Val_Symbolic 9%Z)) Mk_annot :t:
+  ReadReg "cur_privilege" [] (RegVal_Base (Val_Symbolic 2%Z)) Mk_annot :t:
+  Smt (DeclareConst 20%Z (Ty_BitVec 64%N)) Mk_annot :t:
+  ReadReg "satp" [] (RegVal_Base (Val_Symbolic 20%Z)) Mk_annot :t:
+  Smt (DeclareConst 25%Z (Ty_BitVec 64%N)) Mk_annot :t:
+  ReadReg "x11" [] (RegVal_Base (Val_Symbolic 25%Z)) Mk_annot :t:
+  Smt (DefineConst 28%Z (Unop (ZeroExtend 64%N) (Val (Val_Symbolic 6%Z) Mk_annot) Mk_annot)) Mk_annot :t:
+  Smt (DefineConst 34%Z (Unop (ZeroExtend 64%N) (Val (Val_Symbolic 6%Z) Mk_annot) Mk_annot)) Mk_annot :t:
+  Smt (DeclareConst 38%Z Ty_Bool) Mk_annot :t:
+  WriteMem (RegVal_Base (Val_Symbolic 38%Z)) (RegVal_Poison) (RegVal_Base (Val_Symbolic 6%Z)) (RegVal_Base (Val_Symbolic 25%Z)) 8%N None Mk_annot :t:
+  WriteReg "PC" [] (RegVal_Base (Val_Symbolic 5%Z)) Mk_annot :t:
   tnil
 .
