instructions/binary_search_riscv64/a44.v
@@ -4,12 +4,12 @@ Definition a44 : isla_trace :=
   Smt (DeclareConst 0%Z (Ty_BitVec 64%N)) Mk_annot :t:
   ReadReg "PC" [] (RegVal_Base (Val_Symbolic 0%Z)) Mk_annot :t:
   Smt (DefineConst 1%Z (Manyop (Bvmanyarith Bvadd) [Val (Val_Symbolic 0%Z) Mk_annot; Val (Val_Bits (BV 64%N 0x4%Z)) Mk_annot] Mk_annot)) Mk_annot :t:
-  Smt (DeclareConst 17%Z (Ty_BitVec 64%N)) Mk_annot :t:
-  ReadReg "x21" [] (RegVal_Base (Val_Symbolic 17%Z)) Mk_annot :t:
-  Smt (DeclareConst 18%Z (Ty_BitVec 64%N)) Mk_annot :t:
-  ReadReg "x9" [] (RegVal_Base (Val_Symbolic 18%Z)) Mk_annot :t:
-  Smt (DefineConst 19%Z (Binop ((Bvarith Bvsub)) (Val (Val_Symbolic 17%Z) Mk_annot) (Val (Val_Symbolic 18%Z) Mk_annot) Mk_annot)) Mk_annot :t:
-  WriteReg "x10" [] (RegVal_Base (Val_Symbolic 19%Z)) Mk_annot :t:
+  Smt (DeclareConst 2%Z (Ty_BitVec 64%N)) Mk_annot :t:
+  ReadReg "x21" [] (RegVal_Base (Val_Symbolic 2%Z)) Mk_annot :t:
+  Smt (DeclareConst 3%Z (Ty_BitVec 64%N)) Mk_annot :t:
+  ReadReg "x9" [] (RegVal_Base (Val_Symbolic 3%Z)) Mk_annot :t:
+  Smt (DefineConst 4%Z (Binop ((Bvarith Bvsub)) (Val (Val_Symbolic 2%Z) Mk_annot) (Val (Val_Symbolic 3%Z) Mk_annot) Mk_annot)) Mk_annot :t:
+  WriteReg "x10" [] (RegVal_Base (Val_Symbolic 4%Z)) Mk_annot :t:
   WriteReg "PC" [] (RegVal_Base (Val_Symbolic 1%Z)) Mk_annot :t:
   tnil
 .
