instructions/binary_search_riscv64/a70.v
@@ -5,8 +5,8 @@ Definition a70 : isla_trace :=
   Assume (AExp_Binop (Eq) (AExp_Unop (Extract 1%N 1%N) (AExp_Val (AVal_Var "PC" []) Mk_annot) Mk_annot) (AExp_Val (AVal_Bits (BV 1%N 0x0%Z)) Mk_annot) Mk_annot) Mk_annot :t:
   ReadReg "PC" [] (RegVal_Base (Val_Symbolic 0%Z)) Mk_annot :t:
   Smt (DefineConst 1%Z (Manyop (Bvmanyarith Bvadd) [Val (Val_Symbolic 0%Z) Mk_annot; Val (Val_Bits (BV 64%N 0x4%Z)) Mk_annot] Mk_annot)) Mk_annot :t:
-  Smt (DefineConst 4%Z (Manyop (Bvmanyarith Bvadd) [Val (Val_Symbolic 0%Z) Mk_annot; Val (Val_Bits (BV 64%N 0x8%Z)) Mk_annot] Mk_annot)) Mk_annot :t:
-  Smt (DefineConst 5%Z (Unop (Extract 0%N 0%N) (Binop ((Bvarith Bvlshr)) (Val (Val_Symbolic 4%Z) Mk_annot) (Val (Val_Bits (BV 64%N 0x1%Z)) Mk_annot) Mk_annot) Mk_annot)) Mk_annot :t:
-  WriteReg "PC" [] (RegVal_Base (Val_Symbolic 4%Z)) Mk_annot :t:
+  Smt (DefineConst 2%Z (Manyop (Bvmanyarith Bvadd) [Val (Val_Symbolic 0%Z) Mk_annot; Val (Val_Bits (BV 64%N 0x8%Z)) Mk_annot] Mk_annot)) Mk_annot :t:
+  Smt (DefineConst 3%Z (Unop (Extract 0%N 0%N) (Binop ((Bvarith Bvlshr)) (Val (Val_Symbolic 2%Z) Mk_annot) (Val (Val_Bits (BV 64%N 0x1%Z)) Mk_annot) Mk_annot) Mk_annot)) Mk_annot :t:
+  WriteReg "PC" [] (RegVal_Base (Val_Symbolic 2%Z)) Mk_annot :t:
   tnil
 .
