instructions/memcpy_riscv64/ac.v
@@ -4,10 +4,10 @@ Definition ac : isla_trace :=
   Smt (DeclareConst 0%Z (Ty_BitVec 64%N)) Mk_annot :t:
   ReadReg "PC" [] (RegVal_Base (Val_Symbolic 0%Z)) Mk_annot :t:
   Smt (DefineConst 1%Z (Manyop (Bvmanyarith Bvadd) [Val (Val_Symbolic 0%Z) Mk_annot; Val (Val_Bits (BV 64%N 0x4%Z)) Mk_annot] Mk_annot)) Mk_annot :t:
-  Smt (DeclareConst 13%Z (Ty_BitVec 64%N)) Mk_annot :t:
-  ReadReg "x12" [] (RegVal_Base (Val_Symbolic 13%Z)) Mk_annot :t:
-  Smt (DefineConst 14%Z (Manyop (Bvmanyarith Bvadd) [Val (Val_Symbolic 13%Z) Mk_annot; Val (Val_Bits (BV 64%N 0xffffffffffffffff%Z)) Mk_annot] Mk_annot)) Mk_annot :t:
-  WriteReg "x12" [] (RegVal_Base (Val_Symbolic 14%Z)) Mk_annot :t:
+  Smt (DeclareConst 2%Z (Ty_BitVec 64%N)) Mk_annot :t:
+  ReadReg "x12" [] (RegVal_Base (Val_Symbolic 2%Z)) Mk_annot :t:
+  Smt (DefineConst 3%Z (Manyop (Bvmanyarith Bvadd) [Val (Val_Symbolic 2%Z) Mk_annot; Val (Val_Bits (BV 64%N 0xffffffffffffffff%Z)) Mk_annot] Mk_annot)) Mk_annot :t:
+  WriteReg "x12" [] (RegVal_Base (Val_Symbolic 3%Z)) Mk_annot :t:
   WriteReg "PC" [] (RegVal_Base (Val_Symbolic 1%Z)) Mk_annot :t:
   tnil
 .
