instructions/riscv64_test/ac.v
@@ -14,7 +14,7 @@ Definition ac : isla_trace :=
   Assume (AExp_Binop (Eq) (AExp_Unop (Extract 2%N 2%N) (AExp_Val (AVal_Var "misa" [Field "bits"]) Mk_annot) Mk_annot) (AExp_Val (AVal_Bits (BV 1%N 0x1%Z)) Mk_annot) Mk_annot) Mk_annot :t:
   Smt (DeclareConst 1%Z (Ty_BitVec 64%N)) Mk_annot :t:
   Assume (AExp_Binop (Eq) (AExp_Manyop (Bvmanyarith Bvand) [AExp_Val (AVal_Var "mstatus" [Field "bits"]) Mk_annot; AExp_Val (AVal_Bits (BV 64%N 0x20000%Z)) Mk_annot] Mk_annot) (AExp_Val (AVal_Bits (BV 64%N 0x0%Z)) Mk_annot) Mk_annot) Mk_annot :t:
-  Smt (DeclareConst 2%Z (Ty_Enum (Mk_enum_id 3%nat))) Mk_annot :t:
+  Smt (DeclareConst 2%Z (Ty_Enum "Privilege")) Mk_annot :t:
   Assume (AExp_Binop (Eq) (AExp_Val (AVal_Var "cur_privilege" []) Mk_annot) (AExp_Val (AVal_Var "Machine" []) Mk_annot) Mk_annot) Mk_annot :t:
   Smt (DeclareConst 3%Z (Ty_BitVec 64%N)) Mk_annot :t:
   Assume (AExp_Binop (Eq) (AExp_Unop (Extract 2%N 0%N) (AExp_Val (AVal_Var "x2" []) Mk_annot) Mk_annot) (AExp_Val (AVal_Bits (BV 3%N 0x0%Z)) Mk_annot) Mk_annot) Mk_annot :t:
